Notations.v
@@ -2,109 +2,185 @@ Require Export SystemFR.Trees.
 Require Export SystemFR.Syntax.
 Require Export SystemFR.Freshness.
 
-
 Open Scope list.
 
-Declare Custom Entry expr.
-Declare Custom Entry type.
-
-(* Entry point *)
-Notation "'⤳' t" := (fun (fv_id:nat) => t) (at level 100).
-Notation "[| x |]" := (x 0) (x custom expr).
-Notation "[|| x ||]" := (x 0) (x custom type).
-Notation "( x )" := (fun (fv_id:nat) => (x fv_id)) (in custom expr, x custom expr).
-Notation "x" := (⤳ x) (in custom expr at level 0, x ident). 
-Notation "( x )" := (fun (fv_id:nat) => (x fv_id)) (in custom type, x custom type).
-Notation "x" := (⤳ x) (in custom type at level 0, x ident). 
-
-(* Variables (nameless) *)
-Notation "'ft{' v '}'" := (⤳ (fvar v term_var)) (in custom expr, v constr).
-Notation "'lt{' v '}'" := (⤳ (lvar v term_var)) (in custom expr, v constr).
-Notation "'fT{' v '}'" := (⤳ (fvar v type_var)) (in custom expr, v constr).
-Notation "'lT{' v '}'" := (⤳ (lvar v type_var)) (in custom expr, v constr).
 
 
-(* Types *) (* constr and custom entries share the same lexer --' ) (WTF?)*)
-Notation "'Nat'" := (⤳ T_nat) (in custom type).
-Notation "'Unit'" := (⤳ T_unit) (in custom type).
-Notation "'Bool'" := (⤳ T_bool) (in custom type).
-Notation "'⊤'" := (⤳ T_top) (in custom type).
-Notation "'⊥'" := (⤳ T_bot) (in custom type).
 
-Example base_types : ([|| Nat ||], [|| Unit ||], [|| Bool ||], [|| ⊤ ||], [|| ⊥ ||]) = (T_nat, T_unit, T_bool, T_top, T_bot). Proof. reflexivity. Qed.
+(* Untyped embedded language *)
+Module UnTyped.
+  Declare Custom Entry expr.
+  
+  (* Entry point *)
+  Notation "'⤳' t" := (fun (fv_id:nat) => t) (at level 100).
+  Notation "[| x |]" := (x 0) (x custom expr).
+  Notation "( x )" := (fun (fv_id:nat) => (x fv_id)) (in custom expr, x custom expr).
+  Notation "x" := (⤳ x) (in custom expr at level 0, x ident). 
+  (* Variables (nameless) - not used in practice *)
+  Notation "'ft{' v '}'" := (⤳ (fvar v term_var)) (in custom expr, v constr).
+  Notation "'lt{' v '}'" := (⤳ (lvar v term_var)) (in custom expr, v constr).
+  Notation "'fT{' v '}'" := (⤳ (fvar v type_var)) (in custom expr, v constr).
+  Notation "'lT{' v '}'" := (⤳ (lvar v type_var)) (in custom expr, v constr).
 
-Notation "[ t1 ≡ t2 ]" :=
-  (fun fv_id => (T_equiv (t1 fv_id) (t2 fv_id)))
-    (in custom type at level 200,
-     t1 custom expr,
-     t2 custom expr).
+  (* Base terms *)
+  Notation "'0'" := (⤳ zero) (in custom expr).
+  Notation "'1'" := (⤳ (succ zero)) (in custom expr).
+  Notation "'()'" := (⤳ uu) (in custom expr).
+  Notation "'t_true'" := (⤳ttrue) (in custom expr).
+  Notation "'t_false'" := (⤳tfalse) (in custom expr).
+  Notation "'error'" := (notype_err) (in custom expr).
+  Notation "'size' t " := (fun fv_id => (tsize (t fv_id))) (in custom expr at level 0,
+                                                            t custom expr).
+  (* Conditionnal *)
+  Notation "'if' c 'then' t 'else' f" :=
+    (fun fv_id => (ite (c fv_id) (t fv_id) (f fv_id)))
+      (in custom expr at level 1, c custom expr, t custom expr, f custom expr).
 
-Notation "τ1 -> τ2" := (fun fv_id => (T_arrow (τ1 fv_id) (τ2 fv_id))) (in custom type at level 90, right associativity, τ1 custom type, τ2 custom type).
-Notation "x : τ1 -> τ2" :=
-  (fun fv_id => (
-       let x := (fvar fv_id term_var) in
-       (T_arrow (τ1 fv_id) (close 0 (τ2 (S fv_id)) fv_id ))))
-    (in custom type, τ1 custom type at level 85, τ2 custom type at next level, x ident).
+  (* Pairs *)
+  Notation "( t1 , t2 )" :=
+    (fun (fv_id:nat) => (pp (t1 fv_id) (t2 fv_id)))
+      (in custom expr, t1 custom expr, t2 custom expr).
+  Notation "t '._1'" := (fun fv_id => (pi1 (t fv_id))) (in custom expr at level 200, t custom expr).
+  Notation "t '._2'" := (fun fv_id => (pi2 (t fv_id))) (in custom expr at level 200, t custom expr).
 
-Example arrow_type1 : [|| (Nat -> Bool) -> Unit -> ⊤ ||] = T_arrow (T_arrow T_nat T_bool) (T_arrow T_unit T_top).
-Proof. reflexivity. Qed.
-Example arrow_type2 : [|| x : Nat -> y : Nat -> [x ≡ y] ||] = T_arrow T_nat (T_arrow T_nat (T_equiv (lvar 1 term_var) (lvar 0 term_var))).
-Proof. reflexivity. Qed.
+  (* Needs Coq 8.11 to work
+Definition pp_notation (p1 : nat -> tree) (p2 : nat -> tree) : (nat -> tree) :=
+  fun (fv_id : nat) => pp (p1 fv_id) (p2 fv_id).
+Notation "( t1 , .. , t2 , tn )" :=
+  (pp_notation  t1 .. (pp_notation t2 tn) ..)
+    (in custom expr, t1  custom expr, t2 custom expr, tn custom expr, left associativity). *)
+
+  (* Functions *)
+  Notation "'fun' x  => t" := (* non-recursive *)
+    (fun fv_id => (
+         let x := (fvar fv_id term_var) in
+         (notype_lambda (close 0 (t (S fv_id)) fv_id))))
+      (in custom expr at level 100, x ident, t custom expr).
+  Notation "'def_rec' f x => t":= (* recursive *)
+    (fun fv_id => (
+         let f := (fvar fv_id term_var) in
+         let x := (fvar (S fv_id) term_var) in
+         (notype_tfix (close 0 (notype_lambda (close 0 (t (S (S fv_id))) (S fv_id))) fv_id) )))
+      (in custom expr at level 100, f ident, x ident, t custom expr).
+  Notation "'def_rec' f x y => t":=
+    (fun fv_id => (
+         let f := (fvar fv_id term_var) in
+         let x := (fvar (S fv_id) term_var) in
+         let y := (fvar (S (S fv_id)) term_var) in
+         (notype_tfix (close 0 (
+                               notype_lambda (close 0 (notype_lambda (
+                                                           close 0 (t (S(S(S fv_id))))
+                                                                 (S (S fv_id)))) (S fv_id))) fv_id))))
+      (in custom expr at level 100, f ident, x ident, y ident, t custom expr).
+  Notation " t1 t2 " :=
+    (fun fv_id => (app (t1 fv_id) (t2 fv_id)))
+      (in custom expr at level 50, right associativity,
+          t1 custom expr,
+          t2 custom expr).
+
+  (* Naturals *)
+  Notation "'s' t" := (fun fv_id => (succ (t fv_id))) (in custom expr at level 2, t custom expr).
+  Notation "'match' t 'with' '|' '0' => t1 '|' 's' x => t2 'end'" :=
+    (fun (fv_id:nat) => (
+         tmatch (t fv_id)
+                (t1 fv_id)
+                (let x := (fvar fv_id term_var) in (close 0 (t2 (S fv_id)) fv_id))))
+      (in custom expr at level 190, t custom expr, t1 custom expr, t2 custom expr, x ident).
+
+  (* Let expression *)
+  Notation "'let' x := t1 'in' t2" :=
+    (fun (fv_id : nat) => (
+         notype_tlet (t1 fv_id)
+                     (let x := (fvar fv_id term_var) in (close 0 (t2 (S fv_id)) fv_id) )))
+      (in custom expr at level 190, t1 custom expr, t2 custom expr, x ident).
+
+  (* Sum *)
+  Notation "'right' t " :=
+    (fun fv_id => tright (t fv_id))
+      (in custom expr at level 180, right associativity, t custom expr).
+  Notation "'left' t " := 
+    (fun fv_id => tleft (t fv_id))
+      (in custom expr at level 180, right associativity, t custom expr).
+  Notation "'match' t 'with' '|' 'left' l => t1 '|' 'right' r => t2 'end'" :=
+    (fun (fv_id:nat) => (
+         tmatch (t fv_id)
+                (let l  := (fvar fv_id term_var) in (close 0 (t1 (S fv_id)) fv_id))
+                (let r := (fvar fv_id term_var) in (close 0 (t2 (S fv_id)) fv_id))))
+      (in custom expr at level 190, t custom expr, t1 custom expr, t2 custom expr, l ident, r ident).
+
+End UnTyped.
 
 
-Notation "τ1 * τ2" :=(fun fv_id => (T_prod (τ1 fv_id) (τ2 fv_id))) (in custom type at level 90, right associativity, τ1 custom type, τ2 custom type).
+Module Typed.
+  Import UnTyped.
+  Declare Custom Entry type.
 
-Notation "x : τ1 * τ2" :=
-  (fun fv_id => (
-       let x := (fvar fv_id term_var) in
-       (T_prod (τ1 fv_id) (close 0 (τ2 (S fv_id)) fv_id ))))
-    (in custom type, τ1 custom type at level 85, τ2 custom type at level 100, x ident).
+  (* Additionnal entry points *)
+  Notation "[|| x ||]" := (x 0) (x custom type).
+  Notation "( x )" := (fun (fv_id:nat) => (x fv_id)) (in custom type, x custom type).
+  Notation "x" := (⤳ x) (in custom type at level 0, x ident).
 
+  (* Base Types *) 
+  Notation "'Nat'" := (⤳ T_nat) (in custom type).
+  Notation "'Unit'" := (⤳ T_unit) (in custom type).
+  Notation "'Bool'" := (⤳ T_bool) (in custom type).
+  Notation "'⊤'" := (⤳ T_top) (in custom type).
+  Notation "'⊥'" := (⤳ T_bot) (in custom type).
 
-Example prod_type1 : [|| Nat * Bool ||] = T_prod T_nat T_bool.
-Proof. simpl. reflexivity. Qed.
-Example prod_type2 : [|| x : Nat * Bool * Unit ||] = T_prod T_nat (T_prod T_bool T_unit).
-Proof. reflexivity. Qed.
+  (* Additionnal base terms *)
+  Notation "'error' [ T ] " := (fun fv_id => err (T fv_id)) (in custom expr, T custom type).
 
+  (* Equivalence *)
+  Notation "[ t1 ≡ t2 ]" :=
+    (fun fv_id => (T_equiv (t1 fv_id) (t2 fv_id)))
+      (in custom type at level 200,
+          t1 custom expr,
+          t2 custom expr).
 
-Notation "τ1 + τ2" :=
-  (fun fv_id => (T_sum (τ1 fv_id) (τ2 fv_id))) (in custom type at level 95, τ1 custom type, τ2 custom type).
+  (* Arrow type *)
+  Notation "τ1 -> τ2" := (fun fv_id => (T_arrow (τ1 fv_id) (τ2 fv_id))) (in custom type at level 90, right associativity, τ1 custom type, τ2 custom type).
+  Notation "x : τ1 -> τ2" :=
+    (fun fv_id => (
+         let x := (fvar fv_id term_var) in
+         (T_arrow (τ1 fv_id) (close 0 (τ2 (S fv_id)) fv_id ))))
+      (in custom type, τ1 custom type at level 85, τ2 custom type at next level, x ident).
 
-Eval compute in [|| Bool -> Nat + Unit ||].
+  (* Prod type *)
+  Notation "τ1 * τ2" :=(fun fv_id => (T_prod (τ1 fv_id) (τ2 fv_id))) (in custom type at level 90, right associativity, τ1 custom type, τ2 custom type).
+  Notation "x : τ1 * τ2" :=
+    (fun fv_id => (
+         let x := (fvar fv_id term_var) in
+         (T_prod (τ1 fv_id) (close 0 (τ2 (S fv_id)) fv_id ))))
+      (in custom type, τ1 custom type at level 85, τ2 custom type at level 100, x ident).
 
-Example sum_type1 : [|| Bool -> Nat + Unit ||] = T_sum (T_arrow T_bool T_nat) T_unit.
-Proof. reflexivity. Qed.
+  (* Sum type *)
+  Notation "τ1 + τ2" :=
+    (fun fv_id => (T_sum (τ1 fv_id) (τ2 fv_id))) (in custom type at level 95, τ1 custom type, τ2 custom type).
+  Notation "x : τ1 + τ2" :=
+    (fun fv_id => (
+         let x := (fvar fv_id term_var) in
+         (T_sum (τ1 fv_id) (close 0 (τ2 (S fv_id)) fv_id ))))
+      (in custom type, τ1 custom type at level 85, τ2 custom type at level 100, x ident).
 
-Example sum_type2 : [|| Nat + x : Bool -> y : Nat * [x ≡ y] + Nat ||] =  T_sum T_nat (T_arrow T_bool (T_prod T_nat (T_sum (T_equiv (lvar 1 term_var) (lvar 0 term_var)) T_nat))).
-Proof. reflexivity. Qed.
+  (* Refinement types *)
+  Notation "{ x : τ1 | t }" :=
+    (fun fv_id => (
+         let x := (fvar fv_id term_var) in
+         (T_refine (τ1 fv_id) (close 0 (t (S fv_id)) fv_id))))
+      (in custom type at level 200, τ1 custom type, t custom expr, x ident).
+  Notation "{{ x : τ1 | τ2 }}" :=
+    (fun fv_id => (
+         let x := (fvar fv_id term_var) in
+         (T_type_refine (τ1 fv_id) (close 0 (τ2 (S fv_id)) fv_id))))
+      (in custom type at level 200, τ1 custom type, τ2 custom type, x ident).
 
+  (* Union type *)
+  Notation "τ1 ∪ τ2" :=
+    (fun fv_id => (T_union (τ1 fv_id) (τ2 fv_id))) (in custom type at level 190, right associativity, τ1 custom type, τ2 custom type).
 
-Notation "{ x : τ1 | t }" :=
-  (fun fv_id => (
-       let x := (fvar fv_id term_var) in
-       (T_refine (τ1 fv_id) (close 0 (t (S fv_id)) fv_id))))
-    (in custom type at level 200, τ1 custom type, t custom expr, x ident).
-
-Example refine_type1 : [|| { x : Bool | x } ||] = T_refine T_bool (lvar 0 term_var).
-Proof. reflexivity. Qed.
-
-Notation "{{ x : τ1 | τ2 }}" :=
-  (fun fv_id => (
-       let x := (fvar fv_id term_var) in
-       (T_type_refine (τ1 fv_id) (close 0 (τ2 (S fv_id)) fv_id))))
-    (in custom type at level 200, τ1 custom type, τ2 custom type, x ident).
-
-Example refine_by_type1 : [|| {{ x : Bool | [x ≡ x] }} ||] = (T_type_refine T_bool (T_equiv (lvar 0 term_var) (lvar 0 term_var))).
-Proof. reflexivity. Qed.
-
-Notation "τ1 ∪ τ2" :=
-  (fun fv_id => (T_union (τ1 fv_id) (τ2 fv_id))) (in custom type at level 190, right associativity, τ1 custom type, τ2 custom type).
-Notation "τ1 ∩ τ2" :=
-  (fun fv_id => (T_intersection (τ1 fv_id) (τ2 fv_id))) (in custom type at level 170, right associativity, τ1 custom type, τ2 custom type).
-
-Example union_type1 : [|| Nat ∩ Bool ∪ Nat ||] = T_union (T_intersection T_nat T_bool) T_nat.
-Proof. reflexivity. Qed.
-
+  (* Intersection type *)
+  Notation "τ1 ∩ τ2" :=
+    (fun fv_id => (T_intersection (τ1 fv_id) (τ2 fv_id))) (in custom type at level 170, right associativity, τ1 custom type, τ2 custom type).
 (*
 Notation "'forall' x : τ1 . τ2" :=
   (fun fv_id => (
@@ -115,235 +191,34 @@ Notation "'forall' α : 'Type' . τ1 ":=
   (fun fv_id => (
        let α := (fvar fv_id type_var) in
        (T_abs (tclose 0 (τ1 (S fv_id)) fv_id))))
-    (in custom type at level 190, right associativity, τ1 custom type, α ident).
+    (in custom type at level 190, right associativity, τ1 custom type, α ident). *)
 
-(* Tests *)
-Eval compute in
-    [|| Nat ||].
-Eval compute in
-[||  Nat ∩ Bool ∪ Unit ∪ (forall x : Type . Nat) ||]. *)
-                   
+End Typed.
 
+Module Tests.
+  Import UnTyped.
+  Import Typed.  
+  Example base_types : ([|| Nat ||], [|| Unit ||], [|| Bool ||], [|| ⊤ ||], [|| ⊥ ||]) = (T_nat, T_unit, T_bool, T_top, T_bot). Proof. reflexivity. Qed.
+  Example arrow_type1 : [|| (Nat -> Bool) -> Unit -> ⊤ ||] = T_arrow (T_arrow T_nat T_bool) (T_arrow T_unit T_top).
+  Proof. reflexivity. Qed.
+  Example arrow_type2 : [|| x : Nat -> y : Nat -> [x ≡ y] ||] = T_arrow T_nat (T_arrow T_nat (T_equiv (lvar 1 term_var) (lvar 0 term_var))).
+  Proof. reflexivity. Qed.
+  Example prod_type1 : [|| Nat * Bool ||] = T_prod T_nat T_bool.
+  Proof. simpl. reflexivity. Qed.
+  Example prod_type2 : [|| x : Nat * Bool * Unit ||] = T_prod T_nat (T_prod T_bool T_unit).
+  Proof. reflexivity. Qed.
+  Example sum_type1 : [|| Bool -> Nat + Unit ||] = T_sum (T_arrow T_bool T_nat) T_unit.
+  Proof. reflexivity. Qed.
+  Example sum_type2 : [|| Nat + x : Bool -> y : Nat * [x ≡ y] + Nat ||] =  T_sum T_nat (T_arrow T_bool (T_prod T_nat (T_sum (T_equiv (lvar 1 term_var) (lvar 0 term_var)) T_nat))).
+  Proof. reflexivity. Qed.
+  Example refine_type1 : [|| { x : Bool | x } ||] = T_refine T_bool (lvar 0 term_var).
+  Proof. reflexivity. Qed.
+  Example refine_by_type1 : [|| {{ x : Bool | [x ≡ x] }} ||] = (T_type_refine T_bool (T_equiv (lvar 0 term_var) (lvar 0 term_var))).
+  Proof. reflexivity. Qed.
+  Example union_type1 : [|| Nat ∩ Bool ∪ Nat ||] = T_union (T_intersection T_nat T_bool) T_nat.
+  Proof. reflexivity. Qed.
 
-(* Terms *)
-
-(* Base terms *)
-Notation "'0'" := (⤳ zero) (in custom expr).
-Notation "'()'" := (⤳ uu) (in custom expr).
-
-Notation "'error'" := (notype_err) (in custom expr).
-Notation "'error' [ T ] " := (fun fv_id => err (T fv_id)) (in custom expr, T custom type).
-
-(* Pairs *)
-Notation "( t1 , t2 )" :=
-  (fun (fv_id:nat) => (pp (t1 fv_id) (t2 fv_id)))
-  (in custom expr, t1 custom expr, t2 custom expr).
-
-(*
-Needs Coq 8.11 to work
-Definition pp_notation (p1 : nat -> tree) (p2 : nat -> tree) : (nat -> tree) :=
-  fun (fv_id : nat) => pp (p1 fv_id) (p2 fv_id).
-
-Notation "( t1 , .. , t2 , tn )" :=
-  (pp_notation  t1 .. (pp_notation t2 tn) ..)
-    (in custom expr, t1  custom expr, t2 custom expr, tn custom expr, left associativity).
-*)
-
-
-Eval compute in [| (0, ()) |].
-Eval compute in [| ((0,0), (0, (0,0))) |].
-
-
-
-Notation "'fun' => t" :=
-     (fun fv_id => (
-          (notype_lambda (t fv_id))))
-     (in custom expr at level 100, t custom expr).
-
-(*
-Notation "( t1 , t2 )" :=
-  (fun (fv_id:nat) => (pp (t1 fv_id) (t2 fv_id)))
-    (in custom expr, t1 custom expr, t2 custom pairs).
-Notation "t1 , t2" :=
-  (fun (fv_id:nat) => (pp (t1 fv_id) (t2 fv_id)))
-    (in custom pairs at level 190, t1 custom pairs, t2 custom expr, left associativity).
-Notation "t" := t (in custom pairs at level 200, t custom expr).
-          (notype_lambda (close 0 (t (S fv_id)) fv_id))))
-     (in custom expr at level 100, x ident, t custom expr).
-
-     *)
-Notation "'fun' f x  => t" :=
-     (fun fv_id => (
-          let x := (fvar fv_id term_var) in
-          (notype_lambda (close 0 (t (S fv_id)) fv_id))))
-     (in custom expr at level 100, f ident, x ident, t custom expr).
-
-Notation "'fun' x  => t" :=
-     (fun fv_id => (
-          let x := (fvar fv_id term_var) in
-          (notype_lambda (close 0 (t (S fv_id)) fv_id))))
-     (in custom expr at level 100, x ident, t custom expr).
-
-Notation "'def_rec' f x => t":=
-     (fun fv_id => (
-        let f := (fvar fv_id term_var) in
-        let x := (fvar (S fv_id) term_var) in
-        (notype_tfix (close 0 (notype_lambda (close 0 (t (S (S fv_id))) (S fv_id))) fv_id) )))
-     (in custom expr at level 100, f ident, x ident, t custom expr).
-
-Notation "'def_rec' f x y => t":=
-     (fun fv_id => (
-          let f := (fvar fv_id term_var) in
-          let x := (fvar (S fv_id) term_var) in
-          let y := (fvar (S (S fv_id)) term_var) in
-          (notype_tfix (
-             close 0 (
-               notype_lambda (
-                 close 0 (
-                    notype_lambda (
-                        close 0 (
-                          t (S(S(S fv_id))))
-                        (S (S fv_id))))
-                 (S fv_id)))
-             fv_id))))
-     (in custom expr at level 100, f ident, x ident, y ident, t custom expr).
-
-Notation " t1 t2 " :=
-  (fun fv_id => (app (t1 fv_id) (t2 fv_id)))
-    (in custom expr at level 200, left associativity,
-        t1 custom expr,
-        t2 custom expr).
-
-
-
-(* Untyped language *)
-(* --------------------------------------------------------------------- *)
-
-Notation "'()'" := (⤳uu) (in custom expr).
-
-Eval compute in [| () |].
-
-Notation "'size' ( t )" := (fun fv_id => (tsize (t fv_id))) (in custom expr,
-                                         t custom expr).
-
-(* Pairs *)
-
-Notation "t '._1'" := (fun fv_id => (pi1 (t fv_id))) (in custom expr at level 200,
-                                  t custom expr).
-
-
-Notation "t '._2'" := (fun fv_id => (pi2 (t fv_id))) (in custom expr at level 200,
-                                  t custom expr).
-
-(* Booleans *)
-Notation "'t_true'" := (⤳ttrue) (in custom expr).
-Notation "'t_false'" := (⤳tfalse) (in custom expr).
-Notation "'if' c 'then' t 'else' f" := (fun fv_id => (ite (c fv_id) (t fv_id) (f fv_id))) (in custom expr at level 1,
-                                                       c custom expr,
-                                                       t custom expr,
-                                                       f custom expr).
-
-
-(* Naturals *)
-Notation "'1'" := (⤳ (succ zero)) (in custom expr).
-Notation "'s' t" := (fun fv_id => (succ (t fv_id))) (in custom expr at level 2,
-                                 t custom expr).
-
-Notation "'match' t 'with' '|' '0' => t1 '|' 's' x => t2 'end'" :=
-  (fun (fv_id:nat) => (
-       tmatch (t fv_id)
-              (t1 fv_id)
-              (let x := (fvar fv_id term_var) in (close 0 (t2 (S fv_id)) fv_id))))
-  (in custom expr at level 190,
-      t custom expr,
-      t1 custom expr,
-      t2 custom expr,
-      x ident).
-
-Eval compute in
-    [| match 0 with
-         |0 => 1
-         |s n => (
-            match n with
-            | 0 => 0
-            | s n' => n' end) end |].
-
-Definition sfr_plus := [|
- def_rec plus x y =>
- (match x with
-     | 0 => y
-     | s x' => (plus x' y) end)
-|].
-
-Example ex1 : wf sfr_plus 0.
-Proof.
-  repeat step.
-Qed.
-
-(* Let expression *)
-Notation "'let' x := t1 'in' t2" :=
-  (fun (fv_id : nat) => (
-       notype_tlet (t1 fv_id)
-                   (let x := (fvar fv_id term_var) in (close 0 (t2 (S fv_id)) fv_id) )))
-    (in custom expr at level 190,
-        t1 custom expr,
-        t2 custom expr,
-        x ident).
-
-Check
-    [| let n := 1 in (match n with
-                                 | 0 => 1
-                                 | s n' => (match n' with
-                                             | 0 => 1
-                                             | s n'' => ((n, n'),n'') end) end) |].
-
-Eval compute in
-[|
- let plus := (def_rec f x y => (
-     match x with
-      | 0 => y
-      | s x' => (f x' y)
-     end))
- in let fibo := (def_rec f n => (
-        match n with
-         | 0 => 1
-         | s n' => (
-             match n' with
-              | 0 => 1
-              | s n'' => plus (f n') (f n'')
-             end)
-        end))
-    in
-    fibo (s (s (s (s (s 0)))))
-|].
-
-
-(* Sum *)
-Notation "'right' t " :=
-  (fun fv_id => tright (t fv_id))
-  (in custom expr at level 180, right associativity, t custom expr).
-Notation "'left' t " := 
-  (fun fv_id => tleft (t fv_id))
-  (in custom expr at level 180, right associativity, t custom expr).
-
-
-Notation "'match' t 'with' '|' 'left' l => t1 '|' 'right' r => t2 'end'" :=
-  (fun (fv_id:nat) => (
-       tmatch (t fv_id)
-              (let l  := (fvar fv_id term_var) in (close 0 (t1 (S fv_id)) fv_id))
-              (let r := (fvar fv_id term_var) in (close 0 (t2 (S fv_id)) fv_id))))
-  (in custom expr at level 190,
-      t custom expr,
-      t1 custom expr,
-      t2 custom expr,
-      l ident,
-      r ident).
-
-Eval compute in [| fun f x => x |].
-
-Eval compute in [| fun f x => fun g y => x |].
-
-
+End Tests.    
 
 
 
